wip invariant proof for [MsiSv]; finished proving all invariants for children, SFSG!

src/RqRsMsgPred.v
@@ -60,74 +60,76 @@ Section PredMsg.
   Hypotheses (Hiorqs: GoodORqsInit (initsOf sys))
              (Hrrs: RqRsSys dtr sys).
 
+  Definition GoodRqDownPred (rqDown: Id Msg) (P: StatesPred oifc) :=
+    forall oidx,
+      RqDownMsgTo dtr oidx rqDown ->
+      forall pidx,
+        parentIdxOf dtr oidx = Some pidx ->
+        StatesPredR [pidx] P.
+
   Definition GoodRsUpPred (rsUp: Id Msg) (P: StatesPred oifc) :=
     forall oidx,
       RsUpMsgFrom dtr oidx rsUp ->
       StatesPredR (subtreeIndsOf dtr oidx) P.
 
-  Definition GoodRsDownPred (rsDown: Id Msg) (P: StatesPred oifc) :=
-    forall oidx,
-      RsDownMsgTo dtr oidx rsDown ->
-      StatesPredC (subtreeIndsOf dtr oidx) P.
-
-  Definition GoodRqUpPred (rqUp: Id Msg) (P: StatesPred oifc) :=
-    forall oidx,
-      RqUpMsgFrom dtr oidx rqUp ->
-      (In (idOf rqUp) sys.(sys_merqs) \/
-       forall oss orqs, P oss orqs).
-
-  Definition GoodRqDownPred (rqDown: Id Msg) (P: StatesPred oifc) :=
-    forall oidx,
-      RqDownMsgTo dtr oidx rqDown ->
-      forall oss orqs, P oss orqs.
-
   Definition GoodMsgOutPred (P: MsgOutPred oifc) :=
     forall eout: Id Msg,
-      GoodRsUpPred eout (P eout) /\
-      GoodRsDownPred eout (P eout) /\
-      GoodRqUpPred eout (P eout) /\
-      GoodRqDownPred eout (P eout).
+      GoodRqDownPred eout (P eout) /\
+      GoodRsUpPred eout (P eout).
 
   Section Facts.
 
     Ltac disc_rule_custom ::=
       try disc_msg_case.
 
-    Lemma atomic_rqUp_preserves_msg_out_preds:
+    Lemma atomic_rqUp_singleton:
       forall inits ins hst outs eouts,
         Atomic msg_dec inits ins hst outs eouts ->
         forall s1 s2,
           Reachable (steps step_m) sys s1 ->
           steps step_m sys s1 hst s2 ->
-          forall oidx rqUp pidx,
+          forall oidx rqUp,
             In rqUp eouts ->
-            ~ In (idOf rqUp) sys.(sys_merqs) ->
             RqUpMsgFrom dtr oidx rqUp ->
-            parentIdxOf dtr oidx = Some pidx ->
-            forall P oss orqs nost norq,
-              GoodMsgOutPred P ->
-              Forall (fun eout => P eout oss orqs) eouts ->
-              Forall (fun eout => P eout (oss +[pidx <- nost]) (orqs +[pidx <- norq])) eouts.
+            eouts = [rqUp].
     Proof.
       destruct Hrrs as [? [? ?]]; intros.
       eapply atomic_msg_outs_ok in H2; eauto.
       inv H2.
-      - dest_in.
-        repeat constructor.
-        specialize (H9 rqUp); dest.
-        specialize (H9 _ H7).
-        destruct H9.
-        + exfalso; auto.
-        + apply H9.
-      - exfalso; dest_in.
-        disc_rule_conds.
+      - dest_in; reflexivity.
+      - dest_in; reflexivity.
       - exfalso.
-        eapply rqDown_rsUp_inv_msg in H12.
-        rewrite Forall_forall in H12; specialize (H12 _ H5).
-        destruct H12 as [roidx ?].
+        eapply rqDown_rsUp_inv_msg in H8.
+        rewrite Forall_forall in H8; specialize (H8 _ H5).
+        destruct H8 as [roidx ?].
         destruct H2.
         + disc_rule_conds; solve_midx_false.
         + disc_rule_conds.
+    Qed.
+
+    Lemma atomic_rsDown_singleton:
+      forall inits ins hst outs eouts,
+        Atomic msg_dec inits ins hst outs eouts ->
+        forall s1 s2,
+          Reachable (steps step_m) sys s1 ->
+          steps step_m sys s1 hst s2 ->
+          forall oidx rsDown,
+            In rsDown eouts ->
+            RsDownMsgTo dtr oidx rsDown ->
+            eouts = [rsDown].
+    Proof.
+      destruct Hrrs as [? [? ?]]; intros.
+      eapply atomic_msg_outs_ok in H2; eauto.
+      inv H2.
+      - dest_in; reflexivity.
+      - dest_in; reflexivity.
+      - exfalso.
+        eapply rqDown_rsUp_inv_msg in H8.
+        rewrite Forall_forall in H8; specialize (H8 _ H5).
+        destruct H8 as [roidx ?].
+        destruct H2.
+        + disc_rule_conds.
+        + disc_rule_conds; solve_midx_false.
     Qed.
 
     Lemma rqDown_preserves_msg_out_preds:
@@ -141,27 +143,46 @@ Section PredMsg.
           forall P oss orqs nost norq,
             GoodMsgOutPred P ->
             Forall (fun eout => P eout oss orqs) eouts ->
-            Forall (fun eout => P eout (oss +[oidx <- nost]) (orqs +[oidx <- norq])) eouts.
+            Forall (fun eout => P eout (oss +[oidx <- nost]) (orqs +[oidx <- norq]))
+                   (removeOnce (id_dec msg_dec) rqDown eouts).
     Proof.
       destruct Hrrs as [? [? ?]]; intros.
       apply Forall_forall; intros [midx msg] ?.
+      apply removeOnce_In_NoDup in H8;
+        [|apply idsOf_NoDup; eapply rqDownRsUpDisj_NoDup; eauto].
+      dest.
+      
       specialize (H6 (midx, msg)); dest.
-      rewrite Forall_forall in H7; specialize (H7 _ H8).
-      rewrite Forall_forall in H3.
-      pose proof (H3 _ H8).
-      destruct H12 as [cidx ?].
-      destruct H12; [eapply H11; eauto|].
+      rewrite Forall_forall in H7; specialize (H7 _ H9).
+      rewrite Forall_forall in H3; pose proof (H3 _ H9).
+      destruct H11 as [cidx ?].
+      destruct H11.
 
-      specialize (H6 _ H12).
-      eapply H6; [eassumption|].
-      apply OStatesEquivR_add.
+      - specialize (H6 _ H11).
+        red in H11; simpl in *; dest.
+        pose proof (edgeDownTo_Some H _ H12).
+        destruct H13 as [rqUp [rsUp [pidx ?]]]; dest.
+        specialize (H6 _ H15).
+        eapply H6; [eassumption|].
+        apply OStatesEquivR_add.
 
-      eapply rqDownRsUpDisj_in_spec
-        with (eout1:= rqDown) (eout2:= (midx, msg)); eauto.
-      - intro Hx; subst.
-        disc_rule_conds.
-      - left; assumption.
-      - right; assumption.
+        intro Hx; dest_in.
+        eapply rqDownRsUpDisj_in_spec
+          with (oidx1:= cidx) (eout1:= (midx, msg))
+               (oidx2:= oidx) (eout2:= rqDown) in H2; eauto.
+        + elim H2.
+          apply subtreeIndsOf_child_in; [apply H|assumption].
+        + left; red; auto.
+        + red; auto.
+
+      - specialize (H10 _ H11).
+        eapply H10; [eassumption|].
+        apply OStatesEquivR_add.
+
+        eapply rqDownRsUpDisj_in_spec
+          with (eout1:= rqDown) (eout2:= (midx, msg)); eauto.
+        + left; assumption.
+        + right; assumption.
     Qed.
 
     Corollary atomic_rqDown_preserves_msg_out_preds:
@@ -176,7 +197,8 @@ Section PredMsg.
             forall P oss orqs nost norq,
               GoodMsgOutPred P ->
               Forall (fun eout => P eout oss orqs) eouts ->
-              Forall (fun eout => P eout (oss +[oidx <- nost]) (orqs +[oidx <- norq])) eouts.
+              Forall (fun eout => P eout (oss +[oidx <- nost]) (orqs +[oidx <- norq]))
+                     (removeOnce (id_dec msg_dec) rqDown eouts).
     Proof.
       destruct Hrrs as [? [? ?]]; intros.
       eapply atomic_msg_outs_ok in H2; eauto.
@@ -198,53 +220,72 @@ Section PredMsg.
         forall oidx rqTos rsUps Rp,
           SubList rsUps eouts ->
           RqRsDownMatch dtr oidx rqTos (idsOf rsUps) Rp ->
+          (* No RqUp messages in the subtree for the RsUp messages *)
+          Forall (fun eout =>
+                    forall cidx,
+                      RqDownMsgTo dtr cidx eout ->
+                      parentIdxOf dtr cidx <> Some oidx) eouts ->
           forall P oss orqs nost norq,
             GoodMsgOutPred P ->
             Forall (fun eout => P eout oss orqs) eouts ->
-            Forall (fun eout => P eout (oss +[oidx <- nost]) (orqs +[oidx <- norq])) eouts.
+            Forall (fun eout => P eout (oss +[oidx <- nost])
+                                  (orqs +[oidx <- norq]))
+                   (removeL (id_dec msg_dec) eouts rsUps).
     Proof.
       destruct Hrrs as [? [? ?]]; intros.
       apply Forall_forall; intros [midx msg] ?.
-      specialize (H6 (midx, msg)); dest.
-      rewrite Forall_forall in H7; specialize (H7 _ H8).
-      rewrite Forall_forall in H3.
-      pose proof (H3 _ H8).
+      apply removeL_In_NoDup in H9;
+        [|apply idsOf_NoDup; eapply rqDownRsUpDisj_NoDup; eauto].
+      dest.
+      specialize (H7 (midx, msg)); dest.
+      rewrite Forall_forall in H8; specialize (H8 _ H10).
+      rewrite Forall_forall in H3; pose proof (H3 _ H10).
       destruct H12 as [cidx ?].
-      destruct H12; [eapply H11; eauto|].
+      destruct H12.
 
-      specialize (H6 _ H12).
-      eapply H6; [eassumption|].
-      apply OStatesEquivR_add.
+      - specialize (H7 _ H12).
+        rewrite Forall_forall in H6; specialize (H6 _ H10 _ H12).
+        red in H12; simpl in *; dest.
+        pose proof (edgeDownTo_Some H _ H13).
+        destruct H14 as [rqUp [rsUp [pidx ?]]]; dest.
+        specialize (H7 _ H16).
+        eapply H7; [eassumption|].
+        apply OStatesEquivR_add.
+        intro Hx; dest_in; auto.
 
-      assert (exists rcidx rsUp,
-                 parentIdxOf dtr rcidx = Some oidx /\
-                 In rsUp rsUps /\
-                 RsUpMsgFrom dtr rcidx rsUp).
-      { destruct rsUps as [|rsUp rsUps].
-        { exfalso; red in H5; dest.
-          destruct rqTos; [|discriminate]; auto.
+      - specialize (H11 _ H12).
+        eapply H11; [eassumption|].
+        apply OStatesEquivR_add.
+
+        assert (exists rcidx rsUp,
+                   parentIdxOf dtr rcidx = Some oidx /\
+                   In rsUp rsUps /\
+                   RsUpMsgFrom dtr rcidx rsUp).
+        { destruct rsUps as [|rsUp rsUps].
+          { exfalso; red in H5; dest.
+            destruct rqTos; [|discriminate]; auto.
+          }
+          { pose proof (H4 _ (or_introl eq_refl)).
+            eapply RqRsDownMatch_rs_rq in H5; [|left; reflexivity].
+            destruct H5 as [rcidx [down ?]]; dest.
+            specialize (H3 _ H13).
+            destruct H3 as [rcidx0 ?].
+            destruct H3; [destruct H3; exfalso; solve_midx_false|].
+            destruct H3; disc_rule_conds.
+            exists rcidx, rsUp.
+            repeat ssplit; auto.
+            red; auto.
+          }
         }
-        { pose proof (H4 _ (or_introl eq_refl)).
-          eapply RqRsDownMatch_rs_rq in H5; [|left; reflexivity].
-          destruct H5 as [rcidx [down ?]]; dest.
-          specialize (H3 _ H13).
-          destruct H3 as [rcidx0 ?].
-          destruct H3; [destruct H3; exfalso; solve_midx_false|].
-          destruct H3; disc_rule_conds.
-          exists rcidx, rsUp.
-          repeat ssplit; auto.
-          red; auto.
-        }
-      }
-      destruct H13 as [rcidx [rsUp ?]]; dest.
+        destruct H13 as [rcidx [rsUp ?]]; dest.
 
-      destruct (id_dec msg_dec rsUp (midx, msg)); subst.
-      - disc_rule_conds.
-        eapply parent_not_in_subtree; [apply Hrrs|assumption].
-      - eapply outside_parent_out; [apply Hrrs| |eassumption].
-        eapply rqDownRsUpDisj_in_spec
-          with (oidx1:= rcidx) (oidx2:= cidx) in n; eauto;
-          try (red; right; red; eauto).
+        destruct (id_dec msg_dec rsUp (midx, msg)); subst.
+        + disc_rule_conds.
+          eapply parent_not_in_subtree; [apply Hrrs|assumption].
+        + eapply outside_parent_out; [apply Hrrs| |eassumption].
+          eapply rqDownRsUpDisj_in_spec
+            with (oidx1:= rcidx) (oidx2:= cidx) in n; eauto;
+            try (red; right; red; eauto).
     Qed.
 
     Corollary atomic_rsUps_preserves_msg_out_preds:
@@ -257,10 +298,16 @@ Section PredMsg.
             NoDup (idsOf rsUps) ->
             SubList rsUps eouts ->
             RqRsDownMatch dtr oidx rqTos (idsOf rsUps) Rp ->
+            (* No RqUp messages in the subtree for the RsUp messages *)
+            Forall (fun eout =>
+                      forall cidx,
+                        RqDownMsgTo dtr cidx eout ->
+                        parentIdxOf dtr cidx <> Some oidx) eouts ->
             forall P oss orqs nost norq,
               GoodMsgOutPred P ->
               Forall (fun eout => P eout oss orqs) eouts ->
-              Forall (fun eout => P eout (oss +[oidx <- nost]) (orqs +[oidx <- norq])) eouts.
+              Forall (fun eout => P eout (oss +[oidx <- nost]) (orqs +[oidx <- norq]))
+                     (removeL (id_dec msg_dec) eouts rsUps).
     Proof.
       destruct Hrrs as [? [? ?]]; intros.
       eapply atomic_msg_outs_ok in H2; eauto.
@@ -271,7 +318,7 @@ Section PredMsg.
           [red in H7; dest; destruct rqTos; [auto|discriminate]|].
         eapply RqRsDownMatch_rs_rq in H7; [|left; reflexivity].
         destruct H7 as [cidx [down ?]]; dest.
-        destruct H10.
+        destruct H11.
         simpl in *; solve_midx_false.
       - exfalso; destruct rsDown as [rsDown rsm].
         apply SubList_singleton_NoDup in H6; [|apply idsOf_NoDup; assumption].
@@ -279,48 +326,10 @@ Section PredMsg.
           [red in H7; dest; destruct rqTos; [auto|discriminate]|].
         eapply RqRsDownMatch_rs_rq in H7; [|left; reflexivity].
         destruct H7 as [cidx [down ?]]; dest.
-        destruct H10.
+        destruct H11.
         simpl in *; solve_midx_false.
       - eapply rsUps_preserves_msg_out_preds; eauto.
         eapply rqDown_rsUp_inv_msg; eauto.
-    Qed.
-
-    Lemma atomic_rsDown_preserves_msg_out_preds:
-      forall inits ins hst outs eouts,
-        Atomic msg_dec inits ins hst outs eouts ->
-        forall s1 s2,
-          Reachable (steps step_m) sys s1 ->
-          steps step_m sys s1 hst s2 ->
-          forall oidx rsDown,
-            In rsDown eouts ->
-            RsDownMsgTo dtr oidx rsDown ->
-            forall P oss orqs nost norq,
-              GoodMsgOutPred P ->
-              Forall (fun eout => P eout oss orqs) eouts ->
-              Forall (fun eout => P eout (oss +[oidx <- nost]) (orqs +[oidx <- norq])) eouts.
-    Proof.
-      destruct Hrrs as [? [? ?]]; intros.
-      eapply atomic_msg_outs_ok in H2; eauto.
-      inv H2.
-      - exfalso; dest_in.
-        disc_rule_conds.
-      - dest_in.
-        specialize (H7 rsDown); dest.
-        specialize (H5 _ H6).
-        disc_rule_conds.
-        repeat constr_rule_conds.
-        eapply H5; [eassumption|].
-        red; intros; mred.
-        elim H9.
-        apply edgeDownTo_subtreeIndsOf_self_in; [apply Hrrs|].
-        congruence.
-      - exfalso.
-        apply rqDown_rsUp_inv_msg in H10.
-        rewrite Forall_forall in H10; specialize (H10 _ H5).
-        destruct H10 as [cidx ?].
-        destruct H2.
-        + disc_rule_conds.
-        + disc_rule_conds; solve_midx_false.
     Qed.
 
   End Facts.
@@ -366,6 +375,9 @@ Ltac disc_GoodMsgOutPred :=
       is_const down;
       pose proof (edgeDownTo_indsOf _ _ H);
       dest_in; try discriminate
+    | [H: parentIdxOf _ ?oidx = Some ?pidx |- _] => progress simpl in H
+    | [H: parentIdxOf _ ?oidx = Some ?pidx |- _] =>
+      is_const oidx; is_var pidx; inv H
     end.
 
 Close Scope list.
